src/ReactorModel/Determinism/InstStep.lean
@@ -4,7 +4,7 @@ open Classical ReactorType
 
 namespace Execution
 
-theorem InstStep.rcn_not_mem_progress (e : s₁ ⇓ᵢ s₂) : e.rcn.id ∉ s₁.progress := 
+theorem InstStep.rcn_not_mem_progress (e : s₁ ⇓ᵢ s₂) : e.rcn ∉ s₁.progress := 
   sorry -- e.allows.unprocessed
 
 theorem InstStep.preserves_tag (e : s₁ ⇓ᵢ s₂) : s₁.tag = s₂.tag := 
@@ -34,7 +34,7 @@ theorem InstStep.mem_progress_iff :
 
 -- Corollary of `InstStep.mem_progress_iff`.
 theorem InstStep.not_mem_progress :
-  (e : s₁ ⇓ᵢ s₂) → (rcn' ≠ e.rcn) → rcn'.id ∉ s₁.progress → rcn'.id ∉ s₂.progress := 
+  (e : s₁ ⇓ᵢ s₂) → (rcn' ≠ e.rcn) → rcn' ∉ s₁.progress → rcn' ∉ s₂.progress := 
   sorry -- λ h hn hm => (mt h.mem_progress.mp) $ not_or.mpr ⟨hn, hm⟩
 
 -- Corollary of `InstStep.mem_progress`.
@@ -42,20 +42,9 @@ theorem InstStep.monotonic_progress : (s₁ ⇓ᵢ s₂) → rcn' ∈ s₁.progr
   sorry -- (·.mem_progress_iff.mpr $ .inr ·)
 
 -- Corollary of `InstStep.mem_progress`.
-theorem InstStep.rcn_mem_progress : (e : s₁ ⇓ᵢ s₂) → e.rcn.id ∈ s₂.progress := 
+theorem InstStep.rcn_mem_progress : (e : s₁ ⇓ᵢ s₂) → e.rcn ∈ s₂.progress := 
   (·.mem_progress_iff.mpr $ .inl rfl)
 
-theorem identified_changes_equiv_changes {cs : List Change} {o : List (Identified Change)} : 
-  (cs.map ({ id := i, obj := ·}) = o) → (o.map (·.obj) = cs) := by
-  intro h
-  induction cs generalizing o
-  case nil => simp_all
-  case cons hd tl hi =>
-    cases o <;> simp [List.map_cons] at h ⊢
-    case cons hd' tl' =>
-      specialize hi h.right
-      simp [h.left.symm, hi]
-      
 -- If a port is not in the output-dependencies of a given reaction,
 -- then any instantaneous step of the reaction will keep that port
 -- unchanged.
@@ -132,20 +121,20 @@ namespace InstStep
 theorem Skip.equiv : (s₁ ⇓ₛ s₂) → s₁.rtr ≈ s₂.rtr
   | mk .. => .refl
 
-theorem Skip.progress_eq : (e : s₁ ⇓ₛ s₂) → s₂.progress = s₁.progress.insert e.rcn.id
+theorem Skip.progress_eq : (e : s₁ ⇓ₛ s₂) → s₂.progress = s₁.progress.insert e.rcn
   | mk .. => rfl
 
 theorem Skip.progress_mono (e : s₁ ⇓ₛ s₂) : s₁.progress ⊆ s₂.progress := by
   simp [e.progress_eq]
   apply Set.subset_insert
 
-theorem Skip.triggers_iff (e : s₁ ⇓ₛ s₂) : (s₁.Triggers ⟨i, h₁⟩) ↔ (s₂.Triggers ⟨i, h₂⟩) := by 
+theorem Skip.triggers_iff (e : s₁ ⇓ₛ s₂) : (s₁.Triggers i) ↔ (s₂.Triggers i) := by 
   cases e
   case mk rcn _ _ =>
     constructor
     all_goals
       intro h
-      exact h.progress_agnostic (s₁.record_preserves_rtr rcn) (s₁.record_preserves_tag rcn) |>.choose_spec
+      sorry -- exact h.progress_agnostic (s₁.record_preserves_rtr rcn) (s₁.record_preserves_tag rcn) |>.choose_spec
 
 theorem Skip.mem_progress_iff (e : s₁ ⇓ₛ s₂) : 
     (rcn' ∈ s₂.progress) ↔ (rcn' = e.rcn ∨ rcn' ∈ s₁.progress) := by
@@ -153,6 +142,7 @@ theorem Skip.mem_progress_iff (e : s₁ ⇓ₛ s₂) :
 
 theorem Skip.preserves_allows_indep (e₁ : s₁ ⇓ₛ s₂) (e₂ : s₂ ⇓ₛ s₃) (h : e₁.rcn ≮[s₁.rtr] e₂.rcn) : 
     s₁.Allows e₂.rcn where
+  mem := sorry
   unprocessed := Set.not_mem_subset e₁.progress_mono $ e₂.allows_rcn.unprocessed
   deps := by
     intro i hi
@@ -162,9 +152,9 @@ theorem Skip.preserves_allows_indep (e₁ : s₁ ⇓ₛ s₂) (e₂ : s₂ ⇓�
 
 set_option pp.proofs.withType false
 theorem Skip.swap_indep_skip (e₁ : s₁ ⇓ₛ s₂) (e₂ : s₂ ⇓ₛ s₃) (h : e₁.rcn ≮[s₁.rtr] e₂.rcn) : 
-    ∃ (s₂' : _) (f₁ : s₁ ⇓ₛ s₂') (f₂ : s₂' ⇓ₛ s₃), (f₁.rcn.id = e₂.rcn) ∧ (f₂.rcn.id = e₁.rcn) := by 
+    ∃ (s₂' : _) (f₁ : s₁ ⇓ₛ s₂') (f₂ : s₂' ⇓ₛ s₃), (f₁.rcn = e₂.rcn) ∧ (f₂.rcn = e₁.rcn) := by 
   have ha := e₁.preserves_allows_indep e₂ h
-  have ht := e₁.triggers_iff (h₁ := sorry) |>.not.mpr e₂.not_triggers
+  have ht := e₁.triggers_iff.not.mpr e₂.not_triggers
   have e₁' := Skip.mk ha ht
   simp at e₁'
   exists _, e₁'
@@ -172,11 +162,11 @@ theorem Skip.swap_indep_skip (e₁ : s₁ ⇓ₛ s₂) (e₂ : s₂ ⇓ₛ s₃)
         --       Do we need more preservation theorems for `Allows` and `Triggers` first?
 
 theorem Skip.swap_indep_exec (e₁ : s₁ ⇓ₛ s₂) (e₂ : s₂ ⇓ₑ s₃) (h : e₁.rcn ≮[s₁.rtr] e₂.rcn) : 
-    ∃ (s₂' : _) (f₁ : s₁ ⇓ₑ s₂') (f₂ : s₂' ⇓ₛ s₃), (f₁.rcn.id = e₂.rcn) ∧ (f₂.rcn.id = e₁.rcn) := by 
+    ∃ (s₂' : _) (f₁ : s₁ ⇓ₑ s₂') (f₂ : s₂' ⇓ₛ s₃), (f₁.rcn = e₂.rcn) ∧ (f₂.rcn = e₁.rcn) := by 
   sorry
 
 theorem Skip.swap_indep (e₁ : s₁ ⇓ₛ s₂) (e₂ : s₂ ⇓ᵢ s₃) (h : e₁.rcn ≮[s₁.rtr] e₂.rcn) : 
-    ∃ (s₂' : _) (f₁ : s₁ ⇓ᵢ s₂') (f₂ : s₂' ⇓ₛ s₃), (f₁.rcn.id = e₂.rcn) ∧ (f₂.rcn.id = e₁.rcn) := by 
+    ∃ (s₂' : _) (f₁ : s₁ ⇓ᵢ s₂') (f₂ : s₂' ⇓ₛ s₃), (f₁.rcn = e₂.rcn) ∧ (f₂.rcn = e₁.rcn) := by 
   cases e₂
   case skip e₂ =>
     have ⟨_, e₁', e₂', _⟩ := e₁.swap_indep_skip e₂ h
@@ -188,15 +178,15 @@ theorem Skip.swap_indep (e₁ : s₁ ⇓ₛ s₂) (e₂ : s₂ ⇓ᵢ s₃) (h :
 theorem Exec.equiv : (s₁ ⇓ₑ s₂) → s₁.rtr ≈ s₂.rtr
   | mk .. => by simp [State.record_preserves_rtr, s₁.exec_equiv]
 
-theorem Exec.progress_eq : (e : s₁ ⇓ₑ s₂) → s₂.progress = s₁.progress.insert e.rcn.id
+theorem Exec.progress_eq : (e : s₁ ⇓ₑ s₂) → s₂.progress = s₁.progress.insert e.rcn
   | mk .. => rfl
 
 theorem not_Closed (e : s₁ ⇓ᵢ s₂) : ¬s₁.Closed := by
   intro c
   have h := c ▸ e.allows_rcn.unprocessed
   simp [Partial.mem_ids_iff] at h 
-  have := e.rcn.obj?_id_eq_obj ▸ h e.rcn.obj
-  contradiction 
+  sorry -- have := h e.allows.mem.choose
+  -- contradiction 
 
 theorem equiv : (s₁ ⇓ᵢ s₂) → s₁.rtr ≈ s₂.rtr
   | skip e | exec e => e.equiv
@@ -213,7 +203,7 @@ theorem deterministic (e₁ : s ⇓ᵢ s₁) (e₂ : s ⇓ᵢ s₂) (h : e₁.rc
 theorem acyclic (e : s₁ ⇓ᵢ s₂) : e.rcn ≮[s₁.rtr] e.rcn :=
   e.allows_rcn.acyclic
 
-theorem progress_eq : (e : s₁ ⇓ᵢ s₂) → s₂.progress = s₁.progress.insert e.rcn.id
+theorem progress_eq : (e : s₁ ⇓ᵢ s₂) → s₂.progress = s₁.progress.insert e.rcn
   | skip e | exec e => e.progress_eq  
 
 /-
@@ -229,7 +219,7 @@ By cases on e₁ and e₂:
     reduces to a theorem on State.exec?
 -/
 theorem prepend_indep (e₁ : s₁ ⇓ᵢ s₂) (e₂ : s₂ ⇓ᵢ s₃) (h : e₁.rcn ≮[s₁.rtr] e₂.rcn) :
-    ∃ (s₂' : _) (e₁' : s₁ ⇓ᵢ s₂') (e₂' : s₂' ⇓ᵢ s₃), e₁'.rcn.id = e₂.rcn ∧ e₂'.rcn.id = e₁.rcn := by
+    ∃ (s₂' : _) (e₁' : s₁ ⇓ᵢ s₂') (e₂' : s₂' ⇓ᵢ s₃), e₁'.rcn = e₂.rcn ∧ e₂'.rcn = e₁.rcn := by
   cases e₁ 
   case skip e₁ => 
     have ⟨_, e₁', e₂', _⟩ := e₁.swap_indep e₂ h
